Moved split to derived, along with associated lemmas. Also required some new lemmas on subtraction

src/core/DY.Core.Trace.SplitUtils.Derived.fst
@@ -5,28 +5,10 @@ open DY.Core.Trace.Base
 open DY.Core.Trace.SplitUtils
 
 /// This module contains derived functions and lemmas based on
-/// trace_split, trace_concat, trace_subtract, and their properties.
-
-/// Derived functions for trace split
-
-let trace_split_grows (#label_t:Type) (tr:trace_ label_t) (ts:timestamp {ts `on_trace` tr})
-  : Lemma
-    (ensures (
-      let (tr1, e, _) = trace_split tr ts in
-      tr1 <$ tr /\
-      (append_entry tr1 e) <$ tr
-    ))
-  = trace_split_matches_prefix tr ts
+/// trace arithmetic (trace_concat, trace_subtract).
 
 
-let trace_split_at (#a:Type) (tr:trace_ a) (e:trace_entry_ a{entry_exists tr e})
-  : (trace_ a & (e':trace_entry_ a{trace_entry_equiv e e'}) & trace_ a)
-  = let idx = trace_find tr e in
-    let (tr1, e', tr2) = trace_split tr idx in
-    trace_split_get_entry tr idx idx;
-    (tr1, e', tr2)
-
-/// Derived functions for trace arithmetic
+/// Derived properties of trace arithmetic
 
 let trace_subtract_nil (#label_t:Type) (tr:trace_ label_t)
   : Lemma
@@ -58,3 +40,103 @@ let trace_subtract_concat_slices (#label_t:Type) (tr1 tr2 tr3:trace_ label_t)
     [SMTPat ((tr2 <--> tr1) <++> (tr3 <--> tr2))]
   = trace_subtract_concat_left tr1 tr2 (tr3 <--> tr2);
     trace_subtract_concat tr2 tr3
+
+
+/// Splitting a trace at a particular timestamp, getting the entry at that timestamp,
+/// along with the prefix before and suffix after that timestamp.
+/// Derived from trace subtraction.
+
+let trace_split (#label_t:Type) (tr:trace_ label_t) (ts:timestamp{ts `on_trace` tr})
+  : (trace_ label_t & trace_entry_ label_t & trace_ label_t)
+  = let tr1_e = prefix tr (ts + 1) in
+    (init tr1_e, last tr1_e, tr <--> tr1_e)
+
+/// Properties of trace splitting
+
+let trace_split_trace_length (#label_t:Type) (tr:trace_ label_t) (ts:timestamp{ts `on_trace` tr})
+  : Lemma
+    (
+      let (tr1, e, tr2) = trace_split tr ts in
+      trace_length tr1 = ts /\ trace_length tr2 = (trace_length tr) - ts - 1
+    )
+    [SMTPat (trace_split tr ts)]
+  = ()
+
+let trace_split_get_entry (#label_t:Type) (tr:trace_ label_t) (ts:timestamp{ts `on_trace` tr}) (i:timestamp{i `on_trace` tr})
+  : Lemma
+    (
+      let (tr1, e, tr2) = trace_split tr ts in
+      get_entry_at tr i == (
+        if i < ts then get_entry_at tr1 i
+        else if i = ts then e
+        else get_entry_at tr2 (i - ts - 1)
+      )
+    )
+  = let (tr1, e, tr2) = trace_split tr ts in
+    if i < ts then prefix_prefix_eq tr1 (prefix tr (ts + 1)) ts
+    else if i = ts then ()
+    else trace_subtract_get_entry (append_entry tr1 e) tr i
+
+let trace_split_fmap (#a #b:Type) (tr:trace_ a) (ts:timestamp{ts `on_trace` tr}) (f:a -> b)
+  : Lemma
+    (
+      let (tr1, e, tr2) = trace_split tr ts in
+      let (tr1', e', tr2') = trace_split (fmap_trace f tr) ts in
+      fmap_trace f tr1 == tr1' /\
+      fmap_trace_entry f e == e' /\
+      fmap_trace f tr2 == tr2'
+    )
+  = fmap_trace_prefix f tr (ts + 1);
+    trace_subtract_fmap_trace (prefix tr (ts + 1)) tr f
+
+let trace_split_matches_prefix (#label_t:Type) (tr:trace_ label_t) (ts:timestamp {ts `on_trace` tr})
+  : Lemma
+    (
+      let (tr1, e, _) = trace_split tr ts in
+      tr1 == prefix tr ts /\
+      append_entry tr1 e == prefix tr (ts + 1)
+    )
+  = let (tr1, e, _) = trace_split tr ts in
+    prefix_prefix_eq tr1 (prefix tr (ts + 1)) ts
+
+let trace_split_grows (#label_t:Type) (tr:trace_ label_t) (ts:timestamp{ts `on_trace` tr})
+  : Lemma
+    (
+      let (tr1, e, _) = trace_split tr ts in
+      tr1 <$ tr /\
+      (append_entry tr1 e) <$ tr
+    )
+  = trace_split_matches_prefix tr ts
+
+/// trace_split_at is a version of trace_split that allows us to more easily avoid
+/// dealing explicitly with timestamps in proofs, as we do not need to first use the
+/// fact that an entry exists on the trace to find the corresponding timestamp before
+/// splitting at that entry.
+
+let trace_split_at (#a:Type) (tr:trace_ a) (e:trace_entry_ a{entry_exists tr e})
+  : (trace_ a & (e':trace_entry_ a{trace_entry_equiv e e'}) & trace_ a)
+  = let idx = trace_find tr e in
+    let (tr1, e', tr2) = trace_split tr idx in
+    trace_split_get_entry tr idx idx;
+    (tr1, e', tr2)
+
+
+/// Properties relating split with concat and subtract
+
+let trace_split_concat (#label_t:Type) (tr:trace_ label_t) (ts:timestamp{ts `on_trace` tr})
+  : Lemma
+    (
+      let (tr1, e, tr2) = trace_split tr ts in
+       (append_entry tr1 e) <++> tr2 == tr
+    )
+  = trace_concat_subtract (prefix tr (ts + 1)) tr
+
+let trace_subtract_matches_split (#label_t:Type) (tr1 tr2:trace_ label_t)
+  : Lemma
+    (requires tr1 <$ tr2 /\ is_not_empty tr1)
+    (ensures (
+      let (_, _, tl) = trace_split tr2 (trace_length tr1 - 1) in
+      tl == (tr2 <--> tr1)
+    ))
+  = prefix_prefix_eq tr1 tr2 (trace_length tr1)
+
